src/ConcreteEvidence.v
@@ -24,8 +24,8 @@ Inductive EvidenceC: Set :=
 | nnc: N_ID -> BS -> EvidenceC
 | ggc: Plc -> ASP_PARAMS -> BS -> EvidenceC -> EvidenceC
 | hhc: Plc -> ASP_PARAMS -> BS -> Evidence -> EvidenceC
-| eec: Plc -> ASP_PARAMS -> BS -> EvidenceC -> EvidenceC
-| kkc: Plc -> ASP_PARAMS -> Evidence -> EvidenceC
+| eec: Plc -> ASP_PARAMS -> BS -> (*Evidence ->*) EvidenceC -> EvidenceC
+(* | kkc: Plc -> ASP_PARAMS -> Evidence -> EvidenceC *)
 | ssc: EvidenceC -> EvidenceC -> EvidenceC.
 
 (** The Evidence Type associated with a Typed Concrete Evidence value *)
@@ -34,8 +34,8 @@ Fixpoint et_fun (ec:EvidenceC) : Evidence :=
   | mtc => mt
   | ggc p params _ ec' => uu p EXTD params (et_fun ec')
   | hhc p params _ et => uu p COMP params et
-  | eec p params _ ec' => uu p ENCR params mt (* (et_fun ec') *)
-  | kkc p params et' => uu p KILL params et'
+  | eec p params _ ec' => uu p ENCR params (et_fun ec')  (*mt*) (* (et_fun ec') *)
+  (* | kkc p params et' => uu p KILL params et' *)
   | nnc ni _ => nn ni
   | ssc ec1 ec2 => ss (et_fun ec1) (et_fun ec2)
   end.
